examples/bat/BATAltFixCorrect.v
@@ -11,6 +11,7 @@ From ConCert.Execution Require Import BuildUtils.
 From ConCert.Execution Require Import Containers.
 From ConCert.Execution Require Import Serializable.
 From ConCert.Execution Require Import ContractCommon.
+From ConCert.Execution Require Import ResultMonad.
 From ConCert.Examples.BAT Require Import BATCommon.
 From ConCert.Examples.BAT Require Import BATAltFix.
 From ConCert.Examples.EIP20 Require EIP20Token.
@@ -28,20 +29,13 @@ Tactic Notation "contract_simpl" := unfold init in *; cbn in *; contract_simpl r
 
 Ltac destruct_message :=
   repeat match goal with
-  | H : Blockchain.receive _ _ _ _ _ = Some _ |- _ => unfold Blockchain.receive in H; cbn in H
+  | H : Blockchain.receive _ _ _ _ _ = Ok _ |- _ => unfold Blockchain.receive in H; cbn in H
   | msg : option Msg |- _ => destruct msg
   | msg : Msg |- _ => destruct msg
   | msg : EIP20Token.Msg |- _ => destruct msg
-  | H : Blockchain.receive _ _ _ _ None = Some _ |- _ => now contract_simpl
-  | H : receive _ _ _ None = Some _ |- _ => now contract_simpl
+  | H : Blockchain.receive _ _ _ _ None = Ok _ |- _ => now contract_simpl
+  | H : receive _ _ _ None = Ok _ |- _ => now contract_simpl
   end.
-
-Hint Rewrite N.ltb_lt N.ltb_ge N.leb_le N.leb_gt N.eqb_eq N.eqb_neq
-  Nat.ltb_lt Nat.ltb_ge Nat.leb_le Nat.leb_gt
-  Z.leb_le Z.leb_gt
-  Bool.orb_true_iff Bool.orb_false_iff
-  Bool.andb_true_iff Bool.andb_false_iff
-  Bool.negb_false_iff Bool.negb_true_iff : BoolElim.
 (* end hide *)
 
 
@@ -49,7 +43,7 @@ Hint Rewrite N.ltb_lt N.ltb_ge N.leb_le N.leb_gt N.eqb_eq N.eqb_neq
 (** ** Transfer correct *)
 
 Lemma try_transfer_balance_correct : forall prev_state new_state chain ctx to amount new_acts,
-  receive chain ctx prev_state (Some (transfer to amount)) = Some (new_state, new_acts) ->
+  receive chain ctx prev_state (Some (transfer to amount)) = Ok (new_state, new_acts) ->
   EIP20TokenCorrect.transfer_balance_update_correct (token_state prev_state) (token_state new_state) ctx.(ctx_from) to amount = true.
 Proof.
   intros * receive_some.
@@ -58,7 +52,7 @@ Proof.
 Qed.
 
 Lemma try_transfer_preserves_total_supply : forall prev_state new_state chain ctx to amount new_acts,
-  receive chain ctx prev_state (Some (transfer to amount)) = Some (new_state, new_acts) ->
+  receive chain ctx prev_state (Some (transfer to amount)) = Ok (new_state, new_acts) ->
     (total_supply prev_state) = (total_supply new_state).
 Proof.
   intros * receive_some.
@@ -67,7 +61,7 @@ Proof.
 Qed.
 
 Lemma try_transfer_preserves_allowances : forall prev_state new_state chain ctx to amount new_acts,
-  receive chain ctx prev_state (Some (transfer to amount)) = Some (new_state, new_acts) ->
+  receive chain ctx prev_state (Some (transfer to amount)) = Ok (new_state, new_acts) ->
     (allowances prev_state) = (allowances new_state).
 Proof.
   intros * receive_some.
@@ -76,7 +70,7 @@ Proof.
 Qed.
 
 Lemma try_transfer_preserves_other_balances : forall prev_state new_state chain ctx to amount new_acts,
-  receive chain ctx prev_state (Some (transfer to amount)) = Some (new_state, new_acts) ->
+  receive chain ctx prev_state (Some (transfer to amount)) = Ok (new_state, new_acts) ->
     forall account, account <> (ctx_from ctx) -> account <> to ->
       FMap.find account (balances prev_state) = FMap.find account (balances new_state).
 Proof.
@@ -88,7 +82,7 @@ Qed.
 Lemma try_transfer_is_some : forall state chain ctx to amount,
   (ctx_amount ctx <= 0)%Z /\
   amount <= with_default 0 (FMap.find (ctx_from ctx) (balances state))
-    <-> isSome (receive chain ctx state (Some (transfer to amount))) = true.
+    <-> isOk (receive chain ctx state (Some (transfer to amount))) = true.
 Proof.
   intros.
   unfold balances. cbn.
@@ -101,7 +95,7 @@ Qed.
 (** ** Transfer_from correct *)
 
 Lemma try_transfer_from_balance_correct : forall prev_state new_state chain ctx from to amount new_acts,
-  receive chain ctx prev_state (Some (transfer_from from to amount)) = Some (new_state, new_acts) ->
+  receive chain ctx prev_state (Some (transfer_from from to amount)) = Ok (new_state, new_acts) ->
   EIP20TokenCorrect.transfer_balance_update_correct (token_state prev_state) (token_state new_state) from to amount = true /\
   EIP20TokenCorrect.transfer_from_allowances_update_correct (token_state prev_state) (token_state new_state) from ctx.(ctx_from) amount = true.
 Proof.
@@ -111,7 +105,7 @@ Proof.
 Qed.
 
 Lemma try_transfer_from_preserves_total_supply : forall prev_state new_state chain ctx from to amount new_acts,
-  receive chain ctx prev_state (Some (transfer_from from to amount)) = Some (new_state, new_acts) ->
+  receive chain ctx prev_state (Some (transfer_from from to amount)) = Ok (new_state, new_acts) ->
     (total_supply prev_state) = (total_supply new_state).
 Proof.
   intros * receive_some.
@@ -120,7 +114,7 @@ Proof.
 Qed.
 
 Lemma try_transfer_from_preserves_other_balances : forall prev_state new_state chain ctx from to amount new_acts,
-  receive chain ctx prev_state (Some (transfer_from from to amount)) = Some (new_state, new_acts) ->
+  receive chain ctx prev_state (Some (transfer_from from to amount)) = Ok (new_state, new_acts) ->
     forall account, account <> from -> account <> to ->
       FMap.find account (balances prev_state) = FMap.find account (balances new_state).
 Proof.
@@ -130,7 +124,7 @@ Proof.
 Qed.
 
 Lemma try_transfer_from_preserves_other_allowances : forall prev_state new_state chain ctx from to amount new_acts,
-  receive chain ctx prev_state (Some (transfer_from from to amount)) = Some (new_state, new_acts) ->
+  receive chain ctx prev_state (Some (transfer_from from to amount)) = Ok (new_state, new_acts) ->
     forall account, account <> from ->
       FMap.find account (allowances prev_state) = FMap.find account (allowances new_state).
 Proof.
@@ -140,7 +134,7 @@ Proof.
 Qed.
 
 Lemma try_transfer_from_preserves_other_allowance : forall prev_state new_state chain ctx from to amount new_acts,
-  receive chain ctx prev_state (Some (transfer_from from to amount)) = Some (new_state, new_acts) ->
+  receive chain ctx prev_state (Some (transfer_from from to amount)) = Ok (new_state, new_acts) ->
     forall account, account <> (ctx_from ctx) ->
       get_allowance (token_state prev_state) from account = get_allowance (token_state new_state) from account.
 Proof.
@@ -156,7 +150,7 @@ Lemma try_transfer_from_is_some : forall state chain ctx from to amount,
   /\ isSome (get_allowance_ (ctx_from ctx)) = true
   /\ amount <= with_default 0 (FMap.find from (balances state))
   /\ amount <= with_default 0 (get_allowance_ (ctx_from ctx))
-    <-> isSome (receive chain ctx state (Some (transfer_from from to amount))) = true.
+    <-> isOk (receive chain ctx state (Some (transfer_from from to amount))) = true.
 Proof.
   intros * sender_amount_zero.
   unfold balances, allowances, get_allowance_. cbn.
@@ -169,7 +163,7 @@ Qed.
 (** ** Approve correct *)
 
 Lemma try_approve_allowance_correct : forall prev_state new_state chain ctx delegate amount new_acts,
-  receive chain ctx prev_state (Some (approve delegate amount)) = Some (new_state, new_acts) ->
+  receive chain ctx prev_state (Some (approve delegate amount)) = Ok (new_state, new_acts) ->
   EIP20TokenCorrect.approve_allowance_update_correct (token_state new_state) ctx.(ctx_from) delegate amount = true.
 Proof.
   intros * receive_some.
@@ -178,7 +172,7 @@ Proof.
 Qed.
 
 Lemma try_approve_preserves_total_supply : forall prev_state new_state chain ctx delegate amount new_acts,
-  receive chain ctx prev_state (Some (approve delegate amount)) = Some (new_state, new_acts) ->
+  receive chain ctx prev_state (Some (approve delegate amount)) = Ok (new_state, new_acts) ->
     (total_supply prev_state) = (total_supply new_state).
 Proof.
   intros * receive_some.
@@ -187,7 +181,7 @@ Proof.
 Qed.
 
 Lemma try_approve_preserves_balances : forall prev_state new_state chain ctx delegate amount new_acts,
-  receive chain ctx prev_state (Some (approve delegate amount)) = Some (new_state, new_acts) ->
+  receive chain ctx prev_state (Some (approve delegate amount)) = Ok (new_state, new_acts) ->
     (balances prev_state) = (balances new_state).
 Proof.
   intros * receive_some.
@@ -196,7 +190,7 @@ Proof.
 Qed.
 
 Lemma try_approve_preserves_other_allowances : forall prev_state new_state chain ctx delegate amount new_acts,
-  receive chain ctx prev_state (Some (approve delegate amount)) = Some (new_state, new_acts) ->
+  receive chain ctx prev_state (Some (approve delegate amount)) = Ok (new_state, new_acts) ->
     forall account, account <> (ctx_from ctx) ->
       FMap.find account (allowances prev_state) = FMap.find account (allowances new_state).
 Proof.
@@ -206,7 +200,7 @@ Proof.
 Qed.
 
 Lemma try_approve_preserves_other_allowance : forall prev_state new_state chain ctx delegate amount new_acts,
-  receive chain ctx prev_state (Some (approve delegate amount)) = Some (new_state, new_acts) ->
+  receive chain ctx prev_state (Some (approve delegate amount)) = Ok (new_state, new_acts) ->
     forall account, account <> delegate ->
       get_allowance (token_state prev_state) (ctx_from ctx) account = get_allowance (token_state new_state) (ctx_from ctx) account.
 Proof.
@@ -216,7 +210,7 @@ Proof.
 Qed.
 
 Lemma try_approve_is_some : forall state chain ctx delegate amount,
-  (ctx_amount ctx >? 0)%Z = false <-> isSome (receive chain ctx state (Some (approve delegate amount))) = true.
+  (ctx_amount ctx >? 0)%Z = false <-> isOk (receive chain ctx state (Some (approve delegate amount))) = true.
 Proof.
   intros.
   cbn.
@@ -229,7 +223,7 @@ Qed.
 (** ** EIP20 functions only changes token_state *)
 
 Lemma eip_only_changes_token_state : forall prev_state new_state chain ctx m new_acts,
-  receive chain ctx prev_state (Some (tokenMsg m)) = Some (new_state, new_acts) ->
+  receive chain ctx prev_state (Some (tokenMsg m)) = Ok (new_state, new_acts) ->
     prev_state<|token_state := (token_state new_state)|> = new_state.
 Proof.
   intros * receive_some.
@@ -241,7 +235,7 @@ Qed.
 (** ** EIP20 functions not payable *)
 
 Lemma eip20_not_payable : forall prev_state new_state chain ctx m new_acts,
-  receive chain ctx prev_state (Some (tokenMsg m)) = Some (new_state, new_acts) ->
+  receive chain ctx prev_state (Some (tokenMsg m)) = Ok (new_state, new_acts) ->
     (ctx_amount ctx <= 0)%Z.
 Proof.
   intros * receive_some.
@@ -254,7 +248,7 @@ Qed.
 (** ** EIP20 functions produces no acts *)
 
 Lemma eip20_new_acts_correct : forall prev_state new_state chain ctx m new_acts,
-  receive chain ctx prev_state (Some (tokenMsg m)) = Some (new_state, new_acts) ->
+  receive chain ctx prev_state (Some (tokenMsg m)) = Ok (new_state, new_acts) ->
     new_acts = [].
 Proof.
   intros * receive_some.
@@ -267,7 +261,7 @@ Qed.
 (** ** Create_tokens correct *)
 
 Lemma try_create_tokens_balance_correct : forall prev_state new_state chain ctx new_acts,
-  receive chain ctx prev_state (Some create_tokens) = Some (new_state, new_acts) ->
+  receive chain ctx prev_state (Some create_tokens) = Ok (new_state, new_acts) ->
     with_default 0 (FMap.find (ctx_from ctx) (balances prev_state)) =
     with_default 0 (FMap.find (ctx_from ctx) (balances new_state)) - ((Z.to_N (ctx_amount ctx)) * (tokenExchangeRate prev_state)).
 Proof.
@@ -281,7 +275,7 @@ Proof.
 Qed.
 
 Lemma try_create_tokens_total_supply_correct : forall prev_state new_state chain ctx new_acts,
-  receive chain ctx prev_state (Some create_tokens) = Some (new_state, new_acts) ->
+  receive chain ctx prev_state (Some create_tokens) = Ok (new_state, new_acts) ->
     (total_supply prev_state) + ((Z.to_N (ctx_amount ctx)) * (tokenExchangeRate prev_state)) =
     (total_supply new_state).
 Proof.
@@ -290,7 +284,7 @@ Proof.
 Qed.
 
 Lemma try_create_tokens_preserves_other_balances : forall prev_state new_state chain ctx new_acts,
-  receive chain ctx prev_state (Some create_tokens) = Some (new_state, new_acts) ->
+  receive chain ctx prev_state (Some create_tokens) = Ok (new_state, new_acts) ->
     forall account, account <> (ctx_from ctx) ->
       FMap.find account (balances prev_state) = FMap.find account (balances new_state).
 Proof.
@@ -301,7 +295,7 @@ Proof.
 Qed.
 
 Lemma try_create_tokens_preserves_allowances : forall prev_state new_state chain ctx new_acts,
-  receive chain ctx prev_state (Some create_tokens) = Some (new_state, new_acts) ->
+  receive chain ctx prev_state (Some create_tokens) = Ok (new_state, new_acts) ->
     (allowances prev_state) = (allowances new_state).
 Proof.
   intros * receive_some.
@@ -309,7 +303,7 @@ Proof.
 Qed.
 
 Lemma try_create_tokens_only_change_token_state : forall prev_state new_state chain ctx new_acts,
-  receive chain ctx prev_state (Some create_tokens) = Some (new_state, new_acts) ->
+  receive chain ctx prev_state (Some create_tokens) = Ok (new_state, new_acts) ->
     prev_state<|token_state := (token_state new_state)|> = new_state.
 Proof.
   intros * receive_some.
@@ -322,20 +316,26 @@ Lemma try_create_tokens_is_some : forall state chain ctx,
   /\ ((fundingStart state) <= (current_slot chain))%nat
   /\ ((current_slot chain) <= (fundingEnd state))%nat
   /\ (total_supply state) + ((Z.to_N (ctx_amount ctx)) * (tokenExchangeRate state)) <= (tokenCreationCap state)
-    <-> exists x y, receive chain ctx state (Some create_tokens) = Some (x, y).
+    <-> exists x y, receive chain ctx state (Some create_tokens) = Ok (x, y).
 Proof.
   split;
     intros;
     destruct_hyps;
     contract_simpl;
-    autorewrite with BoolElim in *;
-    destruct_or_hyps;
-    try easy;
-    now destruct_address_eq.
+    propify;
+    try easy.
+  - rename H4 into receive_some.
+    destruct_match eqn:funding_active in receive_some.
+    destruct_match eqn:amount_nonnegative in receive_some.
+    destruct_match eqn:cap_not_hit in receive_some; try congruence.
+    all : contract_simpl;
+      propify;
+      destruct_hyps;
+      destruct_or_hyps; try easy.
 Qed.
 
 Lemma try_create_tokens_acts_correct : forall prev_state new_state chain ctx new_acts,
-  receive chain ctx prev_state (Some create_tokens) = Some (new_state, new_acts) ->
+  receive chain ctx prev_state (Some create_tokens) = Ok (new_state, new_acts) ->
     new_acts = [].
 Proof.
   intros.
@@ -343,7 +343,7 @@ Proof.
 Qed.
 
 Lemma try_create_tokens_amount_correct : forall prev_state new_state chain ctx new_acts,
-  receive chain ctx prev_state (Some create_tokens) = Some (new_state, new_acts) ->
+  receive chain ctx prev_state (Some create_tokens) = Ok (new_state, new_acts) ->
     Z.lt 0 ctx.(ctx_amount).
 Proof.
   intros.
@@ -356,17 +356,17 @@ Qed.
 (** ** Finalize correct *)
 
 Lemma try_finalize_isFinalized_correct : forall prev_state new_state chain ctx new_acts,
-  receive chain ctx prev_state (Some finalize) = Some (new_state, new_acts) ->
+  receive chain ctx prev_state (Some finalize) = Ok (new_state, new_acts) ->
     (isFinalized prev_state) = false /\ (isFinalized new_state) = true.
 Proof.
   intros * receive_some.
   contract_simpl.
   split; auto.
-  now autorewrite with BoolElim in *.
+  now propify.
 Qed.
 
 Lemma try_finalize_balance_correct : forall prev_state new_state chain ctx new_acts,
-  receive chain ctx prev_state (Some finalize) = Some (new_state, new_acts) ->
+  receive chain ctx prev_state (Some finalize) = Ok (new_state, new_acts) ->
     with_default 0 (FMap.find prev_state.(batFundDeposit) (balances prev_state)) =
     with_default 0 (FMap.find new_state.(batFundDeposit) (balances new_state)) - new_state.(initSupply).
 Proof.
@@ -380,7 +380,7 @@ Proof.
 Qed.
 
 Lemma try_finalize_total_supply_correct : forall prev_state new_state chain ctx new_acts,
-  receive chain ctx prev_state (Some finalize) = Some (new_state, new_acts) ->
+  receive chain ctx prev_state (Some finalize) = Ok (new_state, new_acts) ->
     (total_supply prev_state) + prev_state.(initSupply) =
     (total_supply new_state).
 Proof.
@@ -389,7 +389,7 @@ Proof.
 Qed.
 
 Lemma try_finalize_preserves_other_balances : forall prev_state new_state chain ctx new_acts,
-  receive chain ctx prev_state (Some finalize) = Some (new_state, new_acts) ->
+  receive chain ctx prev_state (Some finalize) = Ok (new_state, new_acts) ->
     forall account, account <> prev_state.(batFundDeposit) ->
       FMap.find account (balances prev_state) = FMap.find account (balances new_state).
 Proof.
@@ -400,7 +400,7 @@ Proof.
 Qed.
 
 Lemma try_finalize_preserves_allowances : forall prev_state new_state chain ctx new_acts,
-  receive chain ctx prev_state (Some finalize) = Some (new_state, new_acts) ->
+  receive chain ctx prev_state (Some finalize) = Ok (new_state, new_acts) ->
     (allowances prev_state) = (allowances new_state).
 Proof.
   intros * receive_some.
@@ -413,20 +413,20 @@ Lemma try_finalize_is_some : forall state chain ctx,
   /\ (ctx_from ctx) = (fundDeposit state)
   /\ (tokenCreationMin state) <= (total_supply state)
   /\ ((fundingEnd state) < (current_slot chain) \/ (tokenCreationCap state) = (total_supply state))%nat
-    <-> exists x y, receive chain ctx state (Some finalize) = Some (x, y).
+    <-> exists x y, receive chain ctx state (Some finalize) = Ok (x, y).
 Proof.
   split;
     intros;
     destruct_hyps;
     contract_simpl;
-    autorewrite with BoolElim in *;
+    propify;
     destruct_or_hyps;
     try easy;
     now destruct_address_eq.
 Qed.
 
 Lemma try_finalize_acts_correct : forall prev_state new_state chain ctx new_acts,
-  receive chain ctx prev_state (Some finalize) = Some (new_state, new_acts) ->
+  receive chain ctx prev_state (Some finalize) = Ok (new_state, new_acts) ->
     new_acts =
     [act_transfer
       (fundDeposit prev_state)
@@ -442,27 +442,29 @@ Qed.
 (** ** Refund correct *)
 
 Lemma try_refund_balance_correct : forall prev_state new_state chain ctx new_acts,
-  receive chain ctx prev_state (Some refund) = Some (new_state, new_acts) ->
+  receive chain ctx prev_state (Some refund) = Ok (new_state, new_acts) ->
     with_default 0 (FMap.find (ctx_from ctx) (balances new_state)) =
     N.modulo (with_default 0 (FMap.find (ctx_from ctx) (balances prev_state))) prev_state.(tokenExchangeRate).
 Proof.
   intros * receive_some.
   contract_simpl.
+  result_to_option.
   now setoid_rewrite FMap.find_add.
 Qed.
 
 Lemma try_refund_total_supply_correct : forall prev_state new_state chain ctx new_acts,
-  receive chain ctx prev_state (Some refund) = Some (new_state, new_acts) ->
+  receive chain ctx prev_state (Some refund) = Ok (new_state, new_acts) ->
     (total_supply prev_state) - (with_default 0 (FMap.find (ctx_from ctx) (balances prev_state))) +
     N.modulo (with_default 0 (FMap.find (ctx_from ctx) (balances prev_state))) prev_state.(tokenExchangeRate) =
     (total_supply new_state).
 Proof.
   intros * receive_some.
-  now contract_simpl.
+  contract_simpl.
+  now result_to_option.
 Qed.
 
 Lemma try_refund_preserves_other_balances : forall prev_state new_state chain ctx new_acts,
-  receive chain ctx prev_state (Some refund) = Some (new_state, new_acts) ->
+  receive chain ctx prev_state (Some refund) = Ok (new_state, new_acts) ->
     forall account, account <> (ctx_from ctx) ->
       FMap.find account (balances prev_state) = FMap.find account (balances new_state).
 Proof.
@@ -472,7 +474,7 @@ Proof.
 Qed.
 
 Lemma try_refund_preserves_allowances : forall prev_state new_state chain ctx new_acts,
-  receive chain ctx prev_state (Some refund) = Some (new_state, new_acts) ->
+  receive chain ctx prev_state (Some refund) = Ok (new_state, new_acts) ->
     (allowances prev_state) = (allowances new_state).
 Proof.
   intros * receive_some.
@@ -480,7 +482,7 @@ Proof.
 Qed.
 
 Lemma try_refund_only_change_token_state : forall prev_state new_state chain ctx new_acts,
-  receive chain ctx prev_state (Some refund) = Some (new_state, new_acts) ->
+  receive chain ctx prev_state (Some refund) = Ok (new_state, new_acts) ->
     prev_state<|token_state := (token_state new_state)|> = new_state.
 Proof.
   intros * receive_some.
@@ -493,21 +495,22 @@ Lemma try_refund_is_some : forall state chain ctx,
   /\ ((fundingEnd state) < (current_slot chain))%nat
   /\ (total_supply state) < (tokenCreationMin state)
   /\ 0 < with_default 0 (FMap.find (ctx_from ctx) (balances state))
-    <-> exists x y, receive chain ctx state (Some refund) = Some (x, y).
+    <-> exists x y, receive chain ctx state (Some refund) = Ok (x, y).
 Proof.
   split;
     intros;
     destruct_hyps;
     contract_simpl;
-    autorewrite with BoolElim in *;
+    propify;
     destruct_or_hyps;
+    try result_to_option;
     subst; cbn in *;
     try easy;
     now destruct_address_eq.
 Qed.
 
 Lemma try_refund_acts_correct : forall prev_state new_state chain ctx new_acts,
-  receive chain ctx prev_state (Some refund) = Some (new_state, new_acts) ->
+  receive chain ctx prev_state (Some refund) = Ok (new_state, new_acts) ->
     new_acts =
     [act_transfer
       (ctx_from ctx)
@@ -516,6 +519,7 @@ Lemma try_refund_acts_correct : forall prev_state new_state chain ctx new_acts,
 Proof.
   intros.
   contract_simpl.
+  now result_to_option.
 Qed.
 
 
@@ -523,7 +527,7 @@ Qed.
 (** ** Init correct *)
 
 Lemma init_bat_balances_correct : forall state chain ctx setup,
-  init chain ctx setup = Some (state) ->
+  init chain ctx setup = Ok (state) ->
     (balances state) = FMap.empty.
 Proof.
   intros * init_some.
@@ -531,7 +535,7 @@ Proof.
 Qed.
 
 Lemma init_allowances_correct : forall state chain ctx setup,
-  init chain ctx setup = Some (state) ->
+  init chain ctx setup = Ok (state) ->
     (allowances state) = FMap.empty.
 Proof.
   intros * init_some.
@@ -539,7 +543,7 @@ Proof.
 Qed.
 
 Lemma init_isFinalized_correct : forall state chain ctx setup,
-  init chain ctx setup = Some (state) ->
+  init chain ctx setup = Ok (state) ->
     state.(isFinalized) = false.
 Proof.
   intros * init_some.
@@ -547,7 +551,7 @@ Proof.
 Qed.
 
 Lemma init_total_supply_correct : forall state chain ctx setup,
-  init chain ctx setup = Some (state) ->
+  init chain ctx setup = Ok (state) ->
     (total_supply state) = 0.
 Proof.
   intros * init_some.
@@ -555,7 +559,7 @@ Proof.
 Qed.
 
 Lemma init_constants_correct : forall state chain ctx setup,
-  init chain ctx setup = Some (state) ->
+  init chain ctx setup = Ok (state) ->
     state.(fundDeposit) = setup.(_fundDeposit)
     /\ state.(batFundDeposit) = setup.(_batFundDeposit)
     /\ state.(fundingStart) = setup.(_fundingStart)
@@ -574,7 +578,7 @@ Qed.
 (** ** EIP20 functions preserve sum of balances *)
 
 Lemma try_transfer_preserves_balances_sum : forall prev_state new_state chain ctx to amount new_acts,
-  receive chain ctx prev_state (Some (transfer to amount)) = Some (new_state, new_acts) ->
+  receive chain ctx prev_state (Some (transfer to amount)) = Ok (new_state, new_acts) ->
     (sum_balances prev_state) = (sum_balances new_state).
 Proof.
   intros * receive_some.
@@ -583,7 +587,7 @@ Proof.
 Qed.
 
 Lemma try_transfer_from_preserves_balances_sum : forall prev_state new_state chain ctx from to amount new_acts,
-  receive chain ctx prev_state (Some (transfer_from from to amount)) = Some (new_state, new_acts) ->
+  receive chain ctx prev_state (Some (transfer_from from to amount)) = Ok (new_state, new_acts) ->
     (sum_balances prev_state) = (sum_balances new_state).
 Proof.
   intros * receive_some.
@@ -592,7 +596,7 @@ Proof.
 Qed.
 
 Lemma try_approve_preserves_balances_sum : forall prev_state new_state chain ctx delegate amount new_acts,
-  receive chain ctx prev_state (Some (approve delegate amount)) = Some (new_state, new_acts) ->
+  receive chain ctx prev_state (Some (approve delegate amount)) = Ok (new_state, new_acts) ->
     (sum_balances prev_state) = (sum_balances new_state).
 Proof.
   intros * receive_some.
@@ -601,7 +605,7 @@ Proof.
 Qed.
 
 Lemma try_create_tokens_update_balances_sum : forall prev_state new_state chain ctx new_acts,
-  receive chain ctx prev_state (Some create_tokens) = Some (new_state, new_acts) ->
+  receive chain ctx prev_state (Some create_tokens) = Ok (new_state, new_acts) ->
     (sum_balances prev_state) + ((Z.to_N (ctx_amount ctx)) * (tokenExchangeRate prev_state)) = (sum_balances new_state).
 Proof.
   intros * receive_some.
@@ -620,7 +624,7 @@ Proof.
 Qed.
 
 Lemma try_finalize_preserves_balances_sum : forall prev_state new_state chain ctx new_acts,
-  receive chain ctx prev_state (Some finalize) = Some (new_state, new_acts) ->
+  receive chain ctx prev_state (Some finalize) = Ok (new_state, new_acts) ->
     (sum_balances prev_state) + prev_state.(initSupply) = (sum_balances new_state).
 Proof.
   intros * receive_some.
@@ -638,21 +642,23 @@ Proof.
 Qed.
 
 Lemma try_refund_update_balances_sum : forall prev_state new_state chain ctx new_acts,
-  receive chain ctx prev_state (Some refund) = Some (new_state, new_acts) ->
+  receive chain ctx prev_state (Some refund) = Ok (new_state, new_acts) ->
     (sum_balances prev_state) = (sum_balances new_state) + (with_default 0 (FMap.find (ctx_from ctx) (balances prev_state))) -
     N.modulo (with_default 0 (FMap.find (ctx_from ctx) (balances prev_state))) prev_state.(tokenExchangeRate).
 Proof.
   intros * receive_some.
   contract_simpl.
   unfold EIP20Token.sum_balances.
+  result_to_option.
   setoid_rewrite FMap.elements_add_existing; eauto.
-  change n with ((fun '(_, v) => v) (ctx_from ctx, n)).
+  simpl with_default.
+  change t with ((fun '(_, v) => v) (ctx_from ctx, t)).
   rewrite sumN_inv, sumN_swap, fin_maps.map_to_list_delete by auto. cbn.
   now rewrite N.add_comm, N.add_sub.
 Qed.
 
 Lemma init_preserves_balances_sum : forall state chain ctx setup,
-  init chain ctx setup = Some (state) ->
+  init chain ctx setup = Ok (state) ->
     (sum_balances state) = (total_supply state).
 Proof.
   intros * init_some.
@@ -677,18 +683,13 @@ Lemma deployed_implies_constants_valid bstate caddr :
 Proof.
   contract_induction; intros; auto.
   - contract_simpl. cbn.
-    autorewrite with BoolElim in *.
+    propify.
     now destruct_address_eq.
   - destruct_message;
     now contract_simpl.
   - destruct_message;
     now contract_simpl.
-  - instantiate (AddBlockFacts := fun _ _ _ _ _ _ => True).
-    instantiate (DeployFacts := fun _ _ => True).
-    instantiate (CallFacts := fun _ _ _ _ _ => True).
-    unset_all; subst; cbn in *.
-    destruct_chain_step; auto.
-    destruct_action_eval; auto.
+  - solve_facts.
 Qed.
 
 
@@ -707,7 +708,7 @@ Proof.
   assert (receive_sum_balances_eq_total_supply :
           forall prev_state new_state chain ctx msg new_acts,
             total_supply prev_state = sum_balances prev_state ->
-            receive chain ctx prev_state msg = Some (new_state, new_acts) ->
+            receive chain ctx prev_state msg = Ok (new_state, new_acts) ->
             prev_state.(tokenExchangeRate) <> 0 ->
             total_supply new_state = sum_balances new_state).
   - intros prev_state new_state chain ctx msg new_acts IH receive_some exchange_rate_nonzero.
@@ -734,13 +735,8 @@ Proof.
       only 1: instantiate (CallFacts := fun _ _ cstate _ _ => cstate.(tokenExchangeRate) <> 0);
       unfold Blockchain.receive in *; eauto.
     + now apply init_preserves_balances_sum in init_some.
-    + instantiate (AddBlockFacts := fun _ _ _ _ _ _ => True).
-      instantiate (DeployFacts := fun _ _ => True).
-      unset_all; subst.
-      destruct_chain_step; auto.
-      destruct_action_eval; auto.
-      intros ? contract_deployed ?.
-      now apply deployed_implies_constants_valid in contract_deployed as [].
+    + solve_facts.
+      now apply deployed_implies_constants_valid in deployed0 as [].
 Qed.
 
 
@@ -751,7 +747,7 @@ Qed.
     total supply of tokens cannot decrease *)
 Lemma receive_total_supply_increasing : forall prev_state new_state chain ctx msg new_acts,
   ((current_slot chain) <= (fundingEnd prev_state))%nat \/ tokenCreationMin prev_state <= total_supply prev_state->
-  receive chain ctx prev_state msg = Some (new_state, new_acts) ->
+  receive chain ctx prev_state msg = Ok (new_state, new_acts) ->
        (total_supply prev_state) <= (total_supply new_state).
 Proof.
   intros * funding_active receive_some.
@@ -773,7 +769,7 @@ Qed.
 
 (** Constants should never change after after receiving msg *)
 Lemma receive_preserves_constants : forall prev_state new_state chain ctx msg new_acts,
-  receive chain ctx prev_state msg = Some (new_state, new_acts) ->
+  receive chain ctx prev_state msg = Ok (new_state, new_acts) ->
        prev_state.(fundDeposit) = new_state.(fundDeposit)
     /\ prev_state.(batFundDeposit) = new_state.(batFundDeposit)
     /\ prev_state.(fundingStart) = new_state.(fundingStart)
@@ -818,7 +814,7 @@ Qed.
 (** Once the contract is in the finalized state it cannot leave it *)
 Lemma final_is_final : forall prev_state new_state chain ctx msg new_acts,
   (isFinalized prev_state) = true /\
-  receive chain ctx prev_state msg = Some (new_state, new_acts) ->
+  receive chain ctx prev_state msg = Ok (new_state, new_acts) ->
     (isFinalized new_state) = true.
 Proof.
   intros * (finalized & receive_some).
@@ -856,13 +852,13 @@ Proof.
     + apply try_approve_preserves_total_supply in receive_some as supply_unchanged.
       now rewrite supply_unchanged, <- finalized_unchanged in *.
     + contract_simpl.
-      now autorewrite with BoolElim in *.
+      now propify.
     + contract_simpl.
-      autorewrite with BoolElim in *.
+      propify.
       cbn in *.
       now rewrite <- N.nlt_ge in *.
     + contract_simpl.
-      now autorewrite with BoolElim in *.
+      now propify.
 Qed.
 
 
@@ -1161,8 +1157,12 @@ Proof.
              try (apply Z.ge_le, account_balance_nonnegative; eauto).
            clear finalized funding_period_started funding_period_not_over.
            cbn.
-           destruct_match eqn:match_amount; destruct_throw_if match_amount.
-           destruct_match eqn:match_cap; destruct_throw_if match_cap; eauto.
+           destruct_match eqn:receive_some.
+           destruct_match eqn:match_amount in receive_some; destruct_throw_if match_amount.
+           destruct_match eqn:match_cap in receive_some; destruct_throw_if match_cap;
+             injection receive_some as <-; reflexivity.
+           destruct_match eqn:match_amount in receive_some; destruct_throw_if match_amount.
+           destruct_match eqn:match_cap in receive_some; destruct_throw_if match_cap.
         --- (* Prove contradiction between match_amount, match_cap and can_hit_fund_min *)
             apply N.ltb_lt in match_cap.
             apply Z.leb_gt, Z.min_glb_lt_iff in match_amount as [min_left min_right].
@@ -1348,14 +1348,8 @@ Proof.
     destruct action_facts as [? _].
     now destruct_address_eq.
   - now rewrite <- perm.
-  - instantiate (DeployFacts := fun _ _ => True).
-    instantiate (AddBlockFacts := fun _ _ _ _ _ _ => True).
-    unset_all; subst.
-    destruct_chain_step; auto.
-    destruct_action_eval; auto.
-    intros ? contract_deployed ?.
-    cbn.
-    apply deployed_implies_constants_valid in contract_deployed; eauto.
+  - solve_facts.
+    apply deployed_implies_constants_valid in deployed0; eauto.
     now destruct_hyps.
     now constructor.
 Qed.
@@ -1439,13 +1433,7 @@ Proof.
       apply N2Z.is_nonneg.
   - now destruct facts.
   - eapply forall_respects_permutation; eauto.
-  - instantiate (AddBlockFacts := fun _ _ _ _ _ _ => True).
-    instantiate (DeployFacts := fun _ _ => True).
-    unset_all; subst.
-    destruct_chain_step; auto.
-    destruct_action_eval; auto.
-    intros cstate contract_deployed _. cbn.
-    subst. cbn.
+  - solve_facts.
     split.
     + (* Prove call fact: 0 <= ctx_contract_balance ctx *)
       destruct_address_eq; subst; try easy.
@@ -1513,13 +1501,7 @@ Proof.
   - now destruct facts.
   - apply IH in not_finalized. subst.
     now apply Permutation.Permutation_nil in perm.
-  - instantiate (AddBlockFacts := fun _ _ _ _ _ _ => True).
-    instantiate (DeployFacts := fun _ _ => True).
-    unset_all; subst.
-    destruct_chain_step; auto.
-    destruct_action_eval; auto.
-    intros ? contract_deployed ?.
-    subst. cbn.
+  - solve_facts.
     split.
     + eapply bat_no_self_calls'; eauto.
       now constructor.
@@ -1586,8 +1568,8 @@ Proof.
     + apply try_create_tokens_amount_correct in receive_some as payable.
       contract_simpl.
       subst. cbn in *.
-      rename H into requirements_check.
-      rewrite !Bool.orb_false_iff in requirements_check.
+      rename H0 into requirements_check.
+      propify.
       destruct requirements_check as ((not_finalized & _) & _).
       split; intros finalized_state.
       * congruence.
@@ -1624,22 +1606,16 @@ Proof.
         specialize N_div_mod as ?.
         specialize N_mod_le as ?.
         specialize (balance_le_sum_balances (ctx_from ctx) prev_state) as ?.
-        rewrite from_balance in *.
+        result_to_option.
         specialize N_sub_mod_le as ?.
-        rewrite H, <- N2Z.inj_sub, N2Z.inj_add, (N2Z.inj_sub _ n); auto.
+        rewrite H, <- N2Z.inj_sub, N2Z.inj_add, (N2Z.inj_sub _ t); auto.
         rewrite <- Z.sub_sub_distr, <- N2Z.inj_sub, <- N2Z.inj_sub; auto.
-        all:  now eapply N.le_trans.
+          all:  now eapply N.le_trans.
     + now contract_simpl.
   - now destruct facts.
   - now erewrite sumZ_permutation in IH_finalized, IH_funding by eauto.
-  - instantiate (AddBlockFacts := fun _ _ _ _ _ _ => True).
-    instantiate (DeployFacts := fun _ _ => True).
-    unset_all; subst.
-    destruct_chain_step; auto.
-    destruct_action_eval; auto.
-    intros ? contract_deployed ?.
-    subst. cbn.
-    repeat split.
+  - solve_facts.
+    destruct_and_split.
     + now apply Z.ge_le.
     + specialize deployed_implies_constants_valid as
         (cstate' & deployed_state' & _ & _ & exchange_rate_nonzero & _ & _); eauto.
