examples/bat/BATCorrect.v
@@ -11,6 +11,7 @@ From ConCert.Execution Require Import BuildUtils.
 From ConCert.Execution Require Import Containers.
 From ConCert.Execution Require Import Serializable.
 From ConCert.Execution Require Import ContractCommon.
+From ConCert.Execution Require Import ResultMonad.
 From ConCert.Examples.BAT Require Import BATCommon.
 From ConCert.Examples.BAT Require Import BAT.
 From ConCert.Examples.EIP20 Require EIP20Token.
@@ -31,16 +32,9 @@ Ltac destruct_message :=
   | msg : option Msg |- _ => destruct msg
   | msg : Msg |- _ => destruct msg
   | msg : EIP20Token.Msg |- _ => destruct msg
-  | H : Blockchain.receive _ _ _ _ None = Some _ |- _ => now contract_simpl
-  | H : receive _ _ _ None = Some _ |- _ => now contract_simpl
+  | H : Blockchain.receive _ _ _ _ None = Ok _ |- _ => now contract_simpl
+  | H : receive _ _ _ None = Ok _ |- _ => now contract_simpl
   end.
-
-Hint Rewrite N.ltb_lt N.ltb_ge N.leb_le N.leb_gt N.eqb_eq N.eqb_neq
-  Nat.ltb_lt Nat.ltb_ge Nat.leb_le Nat.leb_gt
-  Z.leb_le Z.leb_gt
-  Bool.orb_true_iff Bool.orb_false_iff
-  Bool.andb_true_iff Bool.andb_false_iff
-  Bool.negb_false_iff Bool.negb_true_iff : BoolElim.
 (* end hide *)
 
 
@@ -48,7 +42,7 @@ Hint Rewrite N.ltb_lt N.ltb_ge N.leb_le N.leb_gt N.eqb_eq N.eqb_neq
 (** ** Transfer correct *)
 
 Lemma try_transfer_balance_correct : forall prev_state new_state chain ctx to amount new_acts,
-  receive chain ctx prev_state (Some (transfer to amount)) = Some (new_state, new_acts) ->
+  receive chain ctx prev_state (Some (transfer to amount)) = Ok (new_state, new_acts) ->
   EIP20TokenCorrect.transfer_balance_update_correct (token_state prev_state) (token_state new_state)
     ctx.(ctx_from) to amount = true.
 Proof.
@@ -58,7 +52,7 @@ Proof.
 Qed.
 
 Lemma try_transfer_preserves_total_supply : forall prev_state new_state chain ctx to amount new_acts,
-  receive chain ctx prev_state (Some (transfer to amount)) = Some (new_state, new_acts) ->
+  receive chain ctx prev_state (Some (transfer to amount)) = Ok (new_state, new_acts) ->
     (total_supply prev_state) = (total_supply new_state).
 Proof.
   intros * receive_some.
@@ -67,7 +61,7 @@ Proof.
 Qed.
 
 Lemma try_transfer_preserves_allowances : forall prev_state new_state chain ctx to amount new_acts,
-  receive chain ctx prev_state (Some (transfer to amount)) = Some (new_state, new_acts) ->
+  receive chain ctx prev_state (Some (transfer to amount)) = Ok (new_state, new_acts) ->
     (allowances prev_state) = (allowances new_state).
 Proof.
   intros * receive_some.
@@ -76,7 +70,7 @@ Proof.
 Qed.
 
 Lemma try_transfer_preserves_other_balances : forall prev_state new_state chain ctx to amount new_acts,
-  receive chain ctx prev_state (Some (transfer to amount)) = Some (new_state, new_acts) ->
+  receive chain ctx prev_state (Some (transfer to amount)) = Ok (new_state, new_acts) ->
     forall account, account <> (ctx_from ctx) -> account <> to ->
       FMap.find account (balances prev_state) = FMap.find account (balances new_state).
 Proof.
@@ -88,7 +82,7 @@ Qed.
 Lemma try_transfer_is_some : forall state chain ctx to amount,
   (ctx_amount ctx <= 0)%Z /\
   amount <= with_default 0 (FMap.find (ctx_from ctx) (balances state))
-    <-> isSome (receive chain ctx state (Some (transfer to amount))) = true.
+    <-> isOk (receive chain ctx state (Some (transfer to amount))) = true.
 Proof.
   intros.
   unfold balances. cbn.
@@ -101,7 +95,7 @@ Qed.
 (** ** Transfer_from correct *)
 
 Lemma try_transfer_from_balance_correct : forall prev_state new_state chain ctx from to amount new_acts,
-  receive chain ctx prev_state (Some (transfer_from from to amount)) = Some (new_state, new_acts) ->
+  receive chain ctx prev_state (Some (transfer_from from to amount)) = Ok (new_state, new_acts) ->
   EIP20TokenCorrect.transfer_balance_update_correct (token_state prev_state) (token_state new_state) from to amount = true /\
   EIP20TokenCorrect.transfer_from_allowances_update_correct (token_state prev_state) (token_state new_state) from ctx.(ctx_from) amount = true.
 Proof.
@@ -111,7 +105,7 @@ Proof.
 Qed.
 
 Lemma try_transfer_from_preserves_total_supply : forall prev_state new_state chain ctx from to amount new_acts,
-  receive chain ctx prev_state (Some (transfer_from from to amount)) = Some (new_state, new_acts) ->
+  receive chain ctx prev_state (Some (transfer_from from to amount)) = Ok (new_state, new_acts) ->
     (total_supply prev_state) = (total_supply new_state).
 Proof.
   intros * receive_some.
@@ -120,7 +114,7 @@ Proof.
 Qed.
 
 Lemma try_transfer_from_preserves_other_balances : forall prev_state new_state chain ctx from to amount new_acts,
-  receive chain ctx prev_state (Some (transfer_from from to amount)) = Some (new_state, new_acts) ->
+  receive chain ctx prev_state (Some (transfer_from from to amount)) = Ok (new_state, new_acts) ->
     forall account, account <> from -> account <> to ->
       FMap.find account (balances prev_state) = FMap.find account (balances new_state).
 Proof.
@@ -130,7 +124,7 @@ Proof.
 Qed.
 
 Lemma try_transfer_from_preserves_other_allowances : forall prev_state new_state chain ctx from to amount new_acts,
-  receive chain ctx prev_state (Some (transfer_from from to amount)) = Some (new_state, new_acts) ->
+  receive chain ctx prev_state (Some (transfer_from from to amount)) = Ok (new_state, new_acts) ->
     forall account, account <> from ->
       FMap.find account (allowances prev_state) = FMap.find account (allowances new_state).
 Proof.
@@ -140,7 +134,7 @@ Proof.
 Qed.
 
 Lemma try_transfer_from_preserves_other_allowance : forall prev_state new_state chain ctx from to amount new_acts,
-  receive chain ctx prev_state (Some (transfer_from from to amount)) = Some (new_state, new_acts) ->
+  receive chain ctx prev_state (Some (transfer_from from to amount)) = Ok (new_state, new_acts) ->
     forall account, account <> (ctx_from ctx) ->
       get_allowance (token_state prev_state) from account = get_allowance (token_state new_state) from account.
 Proof.
@@ -156,7 +150,7 @@ Lemma try_transfer_from_is_some : forall state chain ctx from to amount,
   /\ isSome (get_allowance_ (ctx_from ctx)) = true
   /\ amount <= with_default 0 (FMap.find from (balances state))
   /\ amount <= with_default 0 (get_allowance_ (ctx_from ctx))
-    <-> isSome (receive chain ctx state (Some (transfer_from from to amount))) = true.
+    <-> isOk (receive chain ctx state (Some (transfer_from from to amount))) = true.
 Proof.
   intros * amount_zero.
   unfold balances, allowances, get_allowance_. cbn.
@@ -169,7 +163,7 @@ Qed.
 (** ** Approve correct *)
 
 Lemma try_approve_allowance_correct : forall prev_state new_state chain ctx delegate amount new_acts,
-  receive chain ctx prev_state (Some (approve delegate amount)) = Some (new_state, new_acts) ->
+  receive chain ctx prev_state (Some (approve delegate amount)) = Ok (new_state, new_acts) ->
   EIP20TokenCorrect.approve_allowance_update_correct (token_state new_state) ctx.(ctx_from) delegate amount = true.
 Proof.
   intros * receive_some.
@@ -178,7 +172,7 @@ Proof.
 Qed.
 
 Lemma try_approve_preserves_total_supply : forall prev_state new_state chain ctx delegate amount new_acts,
-  receive chain ctx prev_state (Some (approve delegate amount)) = Some (new_state, new_acts) ->
+  receive chain ctx prev_state (Some (approve delegate amount)) = Ok (new_state, new_acts) ->
     (total_supply prev_state) = (total_supply new_state).
 Proof.
   intros * receive_some.
@@ -187,7 +181,7 @@ Proof.
 Qed.
 
 Lemma try_approve_preserves_balances : forall prev_state new_state chain ctx delegate amount new_acts,
-  receive chain ctx prev_state (Some (approve delegate amount)) = Some (new_state, new_acts) ->
+  receive chain ctx prev_state (Some (approve delegate amount)) = Ok (new_state, new_acts) ->
     (balances prev_state) = (balances new_state).
 Proof.
   intros * receive_some.
@@ -196,7 +190,7 @@ Proof.
 Qed.
 
 Lemma try_approve_preserves_other_allowances : forall prev_state new_state chain ctx delegate amount new_acts,
-  receive chain ctx prev_state (Some (approve delegate amount)) = Some (new_state, new_acts) ->
+  receive chain ctx prev_state (Some (approve delegate amount)) = Ok (new_state, new_acts) ->
     forall account, account <> (ctx_from ctx) ->
       FMap.find account (allowances prev_state) = FMap.find account (allowances new_state).
 Proof.
@@ -206,7 +200,7 @@ Proof.
 Qed.
 
 Lemma try_approve_preserves_other_allowance : forall prev_state new_state chain ctx delegate amount new_acts,
-  receive chain ctx prev_state (Some (approve delegate amount)) = Some (new_state, new_acts) ->
+  receive chain ctx prev_state (Some (approve delegate amount)) = Ok (new_state, new_acts) ->
     forall account, account <> delegate ->
       get_allowance (token_state prev_state) (ctx_from ctx) account = get_allowance (token_state new_state) (ctx_from ctx) account.
 Proof.
@@ -216,7 +210,7 @@ Proof.
 Qed.
 
 Lemma try_approve_is_some : forall state chain ctx delegate amount,
-  (ctx_amount ctx >? 0)%Z = false <-> isSome (receive chain ctx state (Some (approve delegate amount))) = true.
+  (ctx_amount ctx >? 0)%Z = false <-> isOk (receive chain ctx state (Some (approve delegate amount))) = true.
 Proof.
   intros.
   cbn.
@@ -229,7 +223,7 @@ Qed.
 (** ** EIP20 functions only changes token_state *)
 
 Lemma eip_only_changes_token_state : forall prev_state new_state chain ctx m new_acts,
-  receive chain ctx prev_state (Some (tokenMsg m)) = Some (new_state, new_acts) ->
+  receive chain ctx prev_state (Some (tokenMsg m)) = Ok (new_state, new_acts) ->
     prev_state<|token_state := (token_state new_state)|> = new_state.
 Proof.
   intros * receive_some.
@@ -241,7 +235,7 @@ Qed.
 (** ** EIP20 functions not payable *)
 
 Lemma eip20_not_payable : forall prev_state new_state chain ctx m new_acts,
-  receive chain ctx prev_state (Some (tokenMsg m)) = Some (new_state, new_acts) ->
+  receive chain ctx prev_state (Some (tokenMsg m)) = Ok (new_state, new_acts) ->
     (ctx_amount ctx <= 0)%Z.
 Proof.
   intros * receive_some.
@@ -254,7 +248,7 @@ Qed.
 (** ** EIP20 functions produces no acts *)
 
 Lemma eip20_new_acts_correct : forall prev_state new_state chain ctx m new_acts,
-  receive chain ctx prev_state (Some (tokenMsg m)) = Some (new_state, new_acts) ->
+  receive chain ctx prev_state (Some (tokenMsg m)) = Ok (new_state, new_acts) ->
     new_acts = [].
 Proof.
   intros * receive_some.
@@ -267,7 +261,7 @@ Qed.
 (** ** Create_tokens correct *)
 
 Lemma try_create_tokens_balance_correct : forall prev_state new_state chain ctx new_acts,
-  receive chain ctx prev_state (Some create_tokens) = Some (new_state, new_acts) ->
+  receive chain ctx prev_state (Some create_tokens) = Ok (new_state, new_acts) ->
     with_default 0 (FMap.find (ctx_from ctx) (balances prev_state)) =
     with_default 0 (FMap.find (ctx_from ctx) (balances new_state)) - ((Z.to_N (ctx_amount ctx)) * (tokenExchangeRate prev_state)).
 Proof.
@@ -281,7 +275,7 @@ Proof.
 Qed.
 
 Lemma try_create_tokens_total_supply_correct : forall prev_state new_state chain ctx new_acts,
-  receive chain ctx prev_state (Some create_tokens) = Some (new_state, new_acts) ->
+  receive chain ctx prev_state (Some create_tokens) = Ok (new_state, new_acts) ->
     (total_supply prev_state) + ((Z.to_N (ctx_amount ctx)) * (tokenExchangeRate prev_state)) =
     (total_supply new_state).
 Proof.
@@ -290,7 +284,7 @@ Proof.
 Qed.
 
 Lemma try_create_tokens_preserves_other_balances : forall prev_state new_state chain ctx new_acts,
-  receive chain ctx prev_state (Some create_tokens) = Some (new_state, new_acts) ->
+  receive chain ctx prev_state (Some create_tokens) = Ok (new_state, new_acts) ->
     forall account, account <> (ctx_from ctx) ->
       FMap.find account (balances prev_state) = FMap.find account (balances new_state).
 Proof.
@@ -301,7 +295,7 @@ Proof.
 Qed.
 
 Lemma try_create_tokens_preserves_allowances : forall prev_state new_state chain ctx new_acts,
-  receive chain ctx prev_state (Some create_tokens) = Some (new_state, new_acts) ->
+  receive chain ctx prev_state (Some create_tokens) = Ok (new_state, new_acts) ->
     (allowances prev_state) = (allowances new_state).
 Proof.
   intros * receive_some.
@@ -309,7 +303,7 @@ Proof.
 Qed.
 
 Lemma try_create_tokens_only_change_token_state : forall prev_state new_state chain ctx new_acts,
-  receive chain ctx prev_state (Some create_tokens) = Some (new_state, new_acts) ->
+  receive chain ctx prev_state (Some create_tokens) = Ok (new_state, new_acts) ->
     prev_state<|token_state := (token_state new_state)|> = new_state.
 Proof.
   intros * receive_some.
@@ -322,19 +316,26 @@ Lemma try_create_tokens_is_some : forall state chain ctx,
   /\ ((fundingStart state) <= (current_slot chain))%nat
   /\ ((current_slot chain) <= (fundingEnd state))%nat
   /\ (total_supply state) + ((Z.to_N (ctx_amount ctx)) * (tokenExchangeRate state)) <= (tokenCreationCap state)
-    <-> exists x y, receive chain ctx state (Some create_tokens) = Some (x, y).
+    <-> exists x y, receive chain ctx state (Some create_tokens) = Ok (x, y).
 Proof.
   split;
     intros;
     destruct_hyps;
     contract_simpl;
-    autorewrite with BoolElim in *;
-    destruct_or_hyps;
+    propify;
     try easy.
+  - rename H4 into receive_some.
+    destruct_match eqn:funding_active in receive_some.
+    destruct_match eqn:amount_nonnegative in receive_some.
+    destruct_match eqn:cap_not_hit in receive_some; try congruence.
+    all : contract_simpl;
+      propify;
+      destruct_hyps;
+      destruct_or_hyps; try easy.
 Qed.
 
 Lemma try_create_tokens_acts_correct : forall prev_state new_state chain ctx new_acts,
-  receive chain ctx prev_state (Some create_tokens) = Some (new_state, new_acts) ->
+  receive chain ctx prev_state (Some create_tokens) = Ok (new_state, new_acts) ->
     new_acts = [].
 Proof.
   intros.
@@ -342,7 +343,7 @@ Proof.
 Qed.
 
 Lemma try_create_tokens_amount_correct : forall prev_state new_state chain ctx new_acts,
-  receive chain ctx prev_state (Some create_tokens) = Some (new_state, new_acts) ->
+  receive chain ctx prev_state (Some create_tokens) = Ok (new_state, new_acts) ->
     Z.lt 0 ctx.(ctx_amount).
 Proof.
   intros.
@@ -355,17 +356,17 @@ Qed.
 (** ** Finalize correct *)
 
 Lemma try_finalize_isFinalized_correct : forall prev_state new_state chain ctx new_acts,
-  receive chain ctx prev_state (Some finalize) = Some (new_state, new_acts) ->
+  receive chain ctx prev_state (Some finalize) = Ok (new_state, new_acts) ->
     (isFinalized prev_state) = false /\ (isFinalized new_state) = true.
 Proof.
   intros * receive_some.
   contract_simpl.
   split; auto.
-  now autorewrite with BoolElim in *.
+  now propify.
 Qed.
 
 Lemma try_finalize_only_change_isFinalized : forall prev_state new_state chain ctx new_acts,
-  receive chain ctx prev_state (Some finalize) = Some (new_state, new_acts) ->
+  receive chain ctx prev_state (Some finalize) = Ok (new_state, new_acts) ->
     prev_state<|isFinalized := (isFinalized new_state)|> = new_state.
 Proof.
   intros * receive_some.
@@ -373,7 +374,7 @@ Proof.
 Qed.
 
 Lemma try_finalize_preserves_total_supply : forall prev_state new_state chain ctx new_acts,
-  receive chain ctx prev_state (Some finalize) = Some (new_state, new_acts) ->
+  receive chain ctx prev_state (Some finalize) = Ok (new_state, new_acts) ->
     (total_supply prev_state) = (total_supply new_state).
 Proof.
   intros * receive_some.
@@ -387,20 +388,20 @@ Lemma try_finalize_is_some : forall state chain ctx,
   /\ (ctx_from ctx) = (fundDeposit state)
   /\ (tokenCreationMin state) <= (total_supply state)
   /\ ((fundingEnd state) < (current_slot chain) \/ (tokenCreationCap state) = (total_supply state))%nat
-    <-> exists x y, receive chain ctx state (Some finalize) = Some (x, y).
+    <-> exists x y, receive chain ctx state (Some finalize) = Ok (x, y).
 Proof.
   split;
     intros;
     destruct_hyps;
     contract_simpl;
-    autorewrite with BoolElim in *;
+    propify;
     destruct_or_hyps;
     try easy;
     now destruct_address_eq.
 Qed.
 
 Lemma try_finalize_acts_correct : forall prev_state new_state chain ctx new_acts,
-  receive chain ctx prev_state (Some finalize) = Some (new_state, new_acts) ->
+  receive chain ctx prev_state (Some finalize) = Ok (new_state, new_acts) ->
     new_acts =
     [act_transfer
       (fundDeposit prev_state)
@@ -416,7 +417,7 @@ Qed.
 (** ** Refund correct *)
 
 Lemma try_refund_balance_correct : forall prev_state new_state chain ctx new_acts,
-  receive chain ctx prev_state (Some refund) = Some (new_state, new_acts) ->
+  receive chain ctx prev_state (Some refund) = Ok (new_state, new_acts) ->
     with_default 0 (FMap.find (ctx_from ctx) (balances new_state)) = 0.
 Proof.
   intros * receive_some.
@@ -425,16 +426,17 @@ Proof.
 Qed.
 
 Lemma try_refund_total_supply_correct : forall prev_state new_state chain ctx new_acts,
-  receive chain ctx prev_state (Some refund) = Some (new_state, new_acts) ->
+  receive chain ctx prev_state (Some refund) = Ok (new_state, new_acts) ->
     (total_supply prev_state) - (with_default 0 (FMap.find (ctx_from ctx) (balances prev_state))) =
     (total_supply new_state).
 Proof.
   intros * receive_some.
-  now contract_simpl.
+  contract_simpl.
+  now result_to_option.
 Qed.
 
 Lemma try_refund_preserves_other_balances : forall prev_state new_state chain ctx new_acts,
-  receive chain ctx prev_state (Some refund) = Some (new_state, new_acts) ->
+  receive chain ctx prev_state (Some refund) = Ok (new_state, new_acts) ->
     forall account, account <> (ctx_from ctx) ->
       FMap.find account (balances prev_state) = FMap.find account (balances new_state).
 Proof.
@@ -444,7 +446,7 @@ Proof.
 Qed.
 
 Lemma try_refund_preserves_allowances : forall prev_state new_state chain ctx new_acts,
-  receive chain ctx prev_state (Some refund) = Some (new_state, new_acts) ->
+  receive chain ctx prev_state (Some refund) = Ok (new_state, new_acts) ->
     (allowances prev_state) = (allowances new_state).
 Proof.
   intros * receive_some.
@@ -452,7 +454,7 @@ Proof.
 Qed.
 
 Lemma try_refund_only_change_token_state : forall prev_state new_state chain ctx new_acts,
-  receive chain ctx prev_state (Some refund) = Some (new_state, new_acts) ->
+  receive chain ctx prev_state (Some refund) = Ok (new_state, new_acts) ->
     prev_state<|token_state := (token_state new_state)|> = new_state.
 Proof.
   intros * receive_some.
@@ -466,21 +468,22 @@ Lemma try_refund_is_some : forall state chain ctx,
   /\ (total_supply state) < (tokenCreationMin state)
   /\ (ctx_from ctx) <> (batFundDeposit state)
   /\ 0 < with_default 0 (FMap.find (ctx_from ctx) (balances state))
-    <-> exists x y, receive chain ctx state (Some refund) = Some (x, y).
+    <-> exists x y, receive chain ctx state (Some refund) = Ok (x, y).
 Proof.
   split;
     intros;
     destruct_hyps;
     contract_simpl;
-    autorewrite with BoolElim in *;
+    propify;
     destruct_or_hyps;
+    try result_to_option;
     subst; cbn in *;
     try easy;
     now destruct_address_eq.
 Qed.
 
 Lemma try_refund_acts_correct : forall prev_state new_state chain ctx new_acts,
-  receive chain ctx prev_state (Some refund) = Some (new_state, new_acts) ->
+  receive chain ctx prev_state (Some refund) = Ok (new_state, new_acts) ->
     new_acts =
     [act_transfer
       (ctx_from ctx)
@@ -489,6 +492,7 @@ Lemma try_refund_acts_correct : forall prev_state new_state chain ctx new_acts,
 Proof.
   intros.
   contract_simpl.
+  now result_to_option.
 Qed.
 
 
@@ -496,7 +500,7 @@ Qed.
 (** ** Init correct *)
 
 Lemma init_bat_balance_correct : forall state chain ctx setup,
-  init chain ctx setup = Some (state) ->
+  init chain ctx setup = Ok (state) ->
     with_default 0 (FMap.find state.(batFundDeposit) (balances state)) = setup.(_batFund).
 Proof.
   intros * init_some.
@@ -505,7 +509,7 @@ Proof.
 Qed.
 
 Lemma init_other_balances_correct : forall state chain ctx setup,
-  init chain ctx setup = Some (state) ->
+  init chain ctx setup = Ok (state) ->
     forall account, account <> state.(batFundDeposit) ->
     with_default 0 (FMap.find account (balances state)) = 0.
 Proof.
@@ -515,7 +519,7 @@ Proof.
 Qed.
 
 Lemma init_allowances_correct : forall state chain ctx setup,
-  init chain ctx setup = Some (state) ->
+  init chain ctx setup = Ok (state) ->
     (allowances state) = FMap.empty.
 Proof.
   intros * init_some.
@@ -523,7 +527,7 @@ Proof.
 Qed.
 
 Lemma init_isFinalized_correct : forall state chain ctx setup,
-  init chain ctx setup = Some (state) ->
+  init chain ctx setup = Ok (state) ->
     state.(isFinalized) = false.
 Proof.
   intros * init_some.
@@ -531,7 +535,7 @@ Proof.
 Qed.
 
 Lemma init_total_supply_correct : forall state chain ctx setup,
-  init chain ctx setup = Some (state) ->
+  init chain ctx setup = Ok (state) ->
     (total_supply state) = setup.(_batFund).
 Proof.
   intros * init_some.
@@ -539,7 +543,7 @@ Proof.
 Qed.
 
 Lemma init_constants_correct : forall state chain ctx setup,
-  init chain ctx setup = Some (state) ->
+  init chain ctx setup = Ok (state) ->
     state.(fundDeposit) = setup.(_fundDeposit)
     /\ state.(batFundDeposit) = setup.(_batFundDeposit)
     /\ state.(fundingStart) = setup.(_fundingStart)
@@ -558,7 +562,7 @@ Qed.
 (** ** Functions preserve sum of balances *)
 
 Lemma try_transfer_preserves_balances_sum : forall prev_state new_state chain ctx to amount new_acts,
-  receive chain ctx prev_state (Some (transfer to amount)) = Some (new_state, new_acts) ->
+  receive chain ctx prev_state (Some (transfer to amount)) = Ok (new_state, new_acts) ->
     (sum_balances prev_state) = (sum_balances new_state).
 Proof.
   intros * receive_some.
@@ -567,7 +571,7 @@ Proof.
 Qed.
 
 Lemma try_transfer_from_preserves_balances_sum : forall prev_state new_state chain ctx from to amount new_acts,
-  receive chain ctx prev_state (Some (transfer_from from to amount)) = Some (new_state, new_acts) ->
+  receive chain ctx prev_state (Some (transfer_from from to amount)) = Ok (new_state, new_acts) ->
     (sum_balances prev_state) = (sum_balances new_state).
 Proof.
   intros * receive_some.
@@ -576,7 +580,7 @@ Proof.
 Qed.
 
 Lemma try_approve_preserves_balances_sum : forall prev_state new_state chain ctx delegate amount new_acts,
-  receive chain ctx prev_state (Some (approve delegate amount)) = Some (new_state, new_acts) ->
+  receive chain ctx prev_state (Some (approve delegate amount)) = Ok (new_state, new_acts) ->
     (sum_balances prev_state) = (sum_balances new_state).
 Proof.
   intros * receive_some.
@@ -585,7 +589,7 @@ Proof.
 Qed.
 
 Lemma try_create_tokens_update_balances_sum : forall prev_state new_state chain ctx new_acts,
-  receive chain ctx prev_state (Some create_tokens) = Some (new_state, new_acts) ->
+  receive chain ctx prev_state (Some create_tokens) = Ok (new_state, new_acts) ->
     (sum_balances prev_state) + ((Z.to_N (ctx_amount ctx)) * (tokenExchangeRate prev_state)) = (sum_balances new_state).
 Proof.
   intros * receive_some.
@@ -603,7 +607,7 @@ Proof.
 Qed.
 
 Lemma try_finalize_preserves_balances_sum : forall prev_state new_state chain ctx new_acts,
-  receive chain ctx prev_state (Some finalize) = Some (new_state, new_acts) ->
+  receive chain ctx prev_state (Some finalize) = Ok (new_state, new_acts) ->
     (sum_balances prev_state) = (sum_balances new_state).
 Proof.
   intros * receive_some.
@@ -611,19 +615,21 @@ Proof.
 Qed.
 
 Lemma try_refund_update_balances_sum : forall prev_state new_state chain ctx new_acts,
-  receive chain ctx prev_state (Some refund) = Some (new_state, new_acts) ->
+  receive chain ctx prev_state (Some refund) = Ok (new_state, new_acts) ->
     (sum_balances prev_state) = (sum_balances new_state) + (with_default 0 (FMap.find (ctx_from ctx) (balances prev_state))).
 Proof.
   intros * receive_some.
   contract_simpl.
   unfold EIP20Token.sum_balances.
+  result_to_option.
   setoid_rewrite FMap.elements_add_existing; eauto.
-  change n with ((fun '(_, v) => v) (ctx_from ctx, n)).
+  simpl with_default.
+  change t with ((fun '(_, v) => v) (ctx_from ctx, t)).
   now rewrite sumN_inv, sumN_swap, fin_maps.map_to_list_delete.
 Qed.
 
 Lemma init_preserves_balances_sum : forall state chain ctx setup,
-  init chain ctx setup = Some (state) ->
+  init chain ctx setup = Ok (state) ->
     (sum_balances state) = (total_supply state).
 Proof.
   intros * receive_some.
@@ -679,7 +685,7 @@ Qed.
     total supply of tokens cannot decrease *)
 Lemma receive_total_supply_increasing : forall prev_state new_state chain ctx msg new_acts,
   ((current_slot chain) <= (fundingEnd prev_state))%nat \/ tokenCreationMin prev_state <= total_supply prev_state->
-  receive chain ctx prev_state msg = Some (new_state, new_acts) ->
+  receive chain ctx prev_state msg = Ok (new_state, new_acts) ->
        (total_supply prev_state) <= (total_supply new_state).
 Proof.
   intros * funding_active receive_some.
@@ -701,7 +707,7 @@ Qed.
 
 (** Constants should never change after after receiving msg *)
 Lemma receive_preserves_constants : forall prev_state new_state chain ctx msg new_acts,
-  receive chain ctx prev_state msg = Some (new_state, new_acts) ->
+  receive chain ctx prev_state msg = Ok (new_state, new_acts) ->
        prev_state.(fundDeposit) = new_state.(fundDeposit)
     /\ prev_state.(batFundDeposit) = new_state.(batFundDeposit)
     /\ prev_state.(fundingStart) = new_state.(fundingStart)
@@ -745,7 +751,7 @@ Qed.
 (** Once the contract is in the finalized state it cannot leave it *)
 Lemma final_is_final : forall prev_state new_state chain ctx msg new_acts,
   (isFinalized prev_state) = true /\
-  receive chain ctx prev_state msg = Some (new_state, new_acts) ->
+  receive chain ctx prev_state msg = Ok (new_state, new_acts) ->
     (isFinalized new_state) = true.
 Proof.
   intros * (finalized & receive_some).
@@ -783,12 +789,12 @@ Proof.
     + apply try_approve_preserves_total_supply in receive_some as supply_unchanged.
       now rewrite supply_unchanged, <- finalized_unchanged in *.
     + contract_simpl.
-      now autorewrite with BoolElim in *.
+      now propify.
     + contract_simpl.
-      autorewrite with BoolElim in *.
+      propify.
       now rewrite <- N.nlt_ge in *.
     + contract_simpl.
-      now autorewrite with BoolElim in *.
+      now propify.
 Qed.
 
 
@@ -1065,7 +1071,7 @@ Proof.
               erewrite (total_balance_eq _ bstate0) by (intros; now rewrite_environment_equiv).
               lia.
         }
-
+        
         (* Now we know that the action is valid we need to evaluate it *)
         evaluate_action BAT.contract; try easy;
           only 1-4: clear fund_deposit_not_contract accounts_not_contracts IHaccounts.
@@ -1085,8 +1091,12 @@ Proof.
              try (apply Z.ge_le, account_balance_nonnegative; eauto).
            clear finalized funding_period_started funding_period_not_over.
            cbn.
-           destruct_match eqn:match_amount; destruct_throw_if match_amount.
-           destruct_match eqn:match_cap; destruct_throw_if match_cap; eauto.
+           destruct_match eqn:receive_some.
+           destruct_match eqn:match_amount in receive_some; destruct_throw_if match_amount.
+           destruct_match eqn:match_cap in receive_some; destruct_throw_if match_cap;
+            injection receive_some as <-; reflexivity.
+           destruct_match eqn:match_amount in receive_some; destruct_throw_if match_amount.
+           destruct_match eqn:match_cap in receive_some; destruct_throw_if match_cap.
          --- (* Prove contradiction between match_amount, match_cap and can_hit_fund_min *)
              apply N.ltb_lt in match_cap.
              apply Z.leb_gt, Z.min_glb_lt_iff in match_amount as [min_left min_right].
@@ -1262,7 +1272,8 @@ Proof.
         rewrite receive_some.
         contract_simpl.
         rename H1 into account_balance_some.
-        replace n with (with_default 0 (FMap.find account (balances cstate))); auto.
+        result_to_option.
+        replace t with (with_default 0 (FMap.find account (balances cstate))); auto.
         now rewrite account_balance_some.
       * repeat split; eauto.
     + now constructor.
